pulse/lib/common/Pulse.Lib.Core.fsti
@@ -495,7 +495,7 @@ val later_elim (p: slprop) : stt_ghost unit emp_inames (later p ** later_credit 
 val later_elim_timeless (p: slprop { timeless p }) : stt_ghost unit emp_inames (later p) (fun _ -> p)
 
 val later_star p q : squash (later (p ** q) == later p ** later q)
-//val later_exists (#t: Type {t}) (f:t->slprop) : squash (later (exists* x. f x) `equiv_pos` (exists* x. later (f x)))
+val later_exists (#t: Type) (f:t->slprop) : stt_ghost unit emp_inames (later (exists* x. f x)) (fun _ -> exists* x. later (f x))
 
 //////////////////////////////////////////////////////////////////////////
 // Equivalence
