pulse/lib/core/PulseCore.Action.fsti
@@ -191,8 +191,8 @@ val later_intro (p:slprop)
 val later_elim (p:slprop)
 : act unit Ghost emp_inames (later p ** later_credit 1) (fun _ -> p)
 
-val later_elim_timeless (p:slprop { timeless p })
-: act unit Ghost emp_inames (later p) (fun _ -> p)
+val implies_elim (p:slprop) (q:slprop { implies p q })
+: act unit Ghost emp_inames p (fun _ -> q)
 
 val buy1 ()
 : stt unit emp (fun _ -> later_credit 1)
