pulse/lib/core/PulseCore.IndirectionTheoryActions.fsti
@@ -47,8 +47,8 @@ val later_intro (e:inames) (p:slprop)
 val later_elim (e:inames) (p:slprop) 
 : ghost_act unit e (later p `star` later_credit 1) (fun _ -> p)
 
-val later_elim_timeless (e:inames) (p:slprop { timeless p })
-: ghost_act unit e (later p) (fun _ -> p)
+val implies_elim (e:inames) (p: slprop) (q:slprop { implies p q })
+: ghost_act unit e p (fun _ -> q)
 
 val buy (e:inames)
 : act unit e emp (fun _ -> later_credit 1)
